list_rec.v
@@ -1,0 +1,29 @@
+Inductive tree (A : Set) : Set :=
+	| node : A -> list (tree A) -> tree A
+.
+
+From Coq Require Import List.
+Import ListNotations.
+
+Definition ind :=
+	forall (A : Set) (P : tree A -> Prop),
+	(forall (a : A)(l : list (tree A)), (forall x, In x l -> P x) -> P (node A a l))
+	-> forall (t : tree A), P t.
+
+Inductive is_sub {A : Set} : tree A -> tree A -> Set :=
+	| sub_refl t : is_sub t t
+	| sub_cons t1 t2 a l :
+		is_sub t1 t2 ->
+		In t2 l ->
+		is_sub t1 (node _ a l)
+.
+
+Theorem tree_ind' : ind.
+Admitted.
+
+Fixpoint sz {A : Set} (t : tree A) : nat :=
+	match t with
+	| node _ _ l => S (fold_right (fun x acc => acc + sz x) 0 l)
+	end.
+
+Print sz.
